Classical_Grounding/Definedness_Translation/Definedness_Translation_Locales.thy
@@ -2,7 +2,7 @@ theory Definedness_Translation_Locales
   imports "Classical_Planning.Classical_Abstract_Syntax"
     Grounding_Classical_Common.Normalization_Definitions
     Classical_Grounding_Utils.PDDL_Sema_Supplement
-    Grounding_Utils.String_Utils
+    Grounding_Utils.String_Utils Grounding_Definedness_Translation.Definedness_Translation_Defs
 begin
 
 section \<open>Definedness Translation Definitions and Locales\<close>
@@ -19,34 +19,6 @@ text \<open>Convert numeric definedness into propositional predicates.
   parameterised by this prefix \<open>pfx\<close>, which is instantiated to \<open>def_prefix\<close> in
   the domain/problem context.\<close>
 
-subsection \<open>Name generation\<close>
-
-definition pne_to_def_atom :: "name \<Rightarrow> 'ent primitive_numeric_expression \<Rightarrow> 'ent atom" where
-  "pne_to_def_atom pfx p = (case p of PNE (Func n) args \<Rightarrow> predAtm (Pred (pfx + n)) args)"
-
-fun def_translate_atom :: "name \<Rightarrow> 'ent atom \<Rightarrow> 'ent atom" where
-  "def_translate_atom pfx (numericEqAtm (FunctionExpr p) (FunctionExpr p')) =
-    (if p = p' then pne_to_def_atom pfx p else numericEqAtm (FunctionExpr p) (FunctionExpr p'))"
-| "def_translate_atom pfx a = a"
-
-definition def_translate_fmla :: "name \<Rightarrow> 'ent atom formula \<Rightarrow> 'ent atom formula" where
-  "def_translate_fmla pfx f = map_formula (def_translate_atom pfx) f"
-
-subsection \<open>Collecting the PNEs of an effect\<close>
-
-definition rhs_pnes_num_eff :: "'ent numeric_effect \<Rightarrow> 'ent primitive_numeric_expression list" where
-  "rhs_pnes_num_eff eff = (case eff of
-    NumericEffect _ _ e \<Rightarrow> enumerate_primitive_numeric_expressions e)"
-
-fun rhs_pnes_eff :: "'ent ast_effect \<Rightarrow> 'ent primitive_numeric_expression list" where
-  "rhs_pnes_eff (Effect _ _ ne) = concat (map rhs_pnes_num_eff ne)"
-
-definition lhs_pnes_num_eff :: "'ent numeric_effect \<Rightarrow> 'ent primitive_numeric_expression list" where
-  "lhs_pnes_num_eff eff = (case eff of
-    NumericEffect numeric_effect_op.Assign p _ \<Rightarrow> [p] | _ \<Rightarrow> [])"
-
-fun lhs_pnes_eff :: "'ent ast_effect \<Rightarrow> 'ent primitive_numeric_expression list" where
-  "lhs_pnes_eff (Effect _ _ ne) = concat (map lhs_pnes_num_eff ne)"
 
 subsection \<open>Action translation\<close>
 
@@ -60,27 +32,7 @@ fun def_translate_ac :: "name \<Rightarrow> ast_classical_action_schema \<Righta
          new_ads = map Atom new_eff_atoms @ ads
      in SimpleActionSchema h (SimpleActionBody new_pre (Effect new_ads dls neffs)))"
 
-definition def_predicate_decl :: "name \<Rightarrow> function_decl \<Rightarrow> predicate_decl" where
-  "def_predicate_decl pfx d = (case d of FuncDecl (Func n) ts \<Rightarrow> PredDecl (Pred (pfx + n)) ts)"
 
-text \<open>Extract from an initial-state function assignment
-  \<open>(= (f args) c)\<close> the definedness fact \<open>Defined_f args\<close>.\<close>
-
-definition init_def_fact :: "name \<Rightarrow> object atom formula \<Rightarrow> object atom formula option" where
-  "init_def_fact pfx f = (case f of
-      Atom (numericEqAtm (FunctionExpr l) (ConstantExpr _)) \<Rightarrow> Some (Atom (pne_to_def_atom pfx l))
-    | _ \<Rightarrow> None)"
-
-subsection \<open>Domain-fresh prefix\<close>
-
-context domain_signature begin
-
-text \<open>A prefix fresh w.r.t. the declared predicate names, extended with the
-  \<open>Defined_\<close> token. Freshness follows from \<open>safe_prefix_correct\<close>.\<close>
-
-definition "def_prefix \<equiv> safe_prefix pred_names + STR ''Defined_''"
-
-end
 
 subsection \<open>Domain and problem translation\<close>
 
