Grounding_Common/Type_Normalization/Type_Normalization_Signature.thy
@@ -1,0 +1,131 @@
+theory Type_Normalization_Signature
+  imports "Continuous_Planning.Signatures"
+    Grounding_Common.Signature_Normalization
+    Grounding_Common.Formula_Utils
+    Grounding_Utils.Graph_Funs
+    Grounding_Utils.String_Utils
+begin
+
+section \<open>Signature-level detyping (reusable)\<close>
+
+text \<open>The AST-agnostic part of type normalization: the detyping helper functions over a PDDL
+  domain/problem \<^emph>\<open>signature\<close>, the detyped predicate/function/object lists, and the parallel \<open>*2\<close>
+  signature-locale hierarchy relating a typed signature to its detyped counterpart. These mention only
+  the shared signature and the shared action AST (\<open>ActionHead\<close>/\<open>SimpleActionBody\<close> from
+  Continuous_Planning), so they are reusable by any grounder. The classical-AST counterparts
+  (\<open>detype_classical_ac\<close>, \<open>detype_classical_dom\<close>/\<open>prob\<close>, the \<open>ast_classical_*2\<close> locales) live in
+  \<open>Classical_Grounding.Type_Normalization_Locales\<close>.\<close>
+
+context domain_signature
+begin
+
+  definition pred_for_type :: "name \<Rightarrow> predicate" where
+      "pred_for_type t \<equiv> Pred (safe_prefix pred_names + (STR ''type_'' + t))"
+
+  fun type_pred :: "name \<Rightarrow> predicate_decl" where
+      "type_pred t = PredDecl (pred_for_type t) [\<omega>]"
+
+  (* if multiple inheritance exists, there are duplicates *)
+  abbreviation "type_names \<equiv> remdups (STR ''object'' # map fst ty_decl)"
+
+  definition type_preds :: "predicate_decl list" where
+    "type_preds \<equiv> map type_pred type_names"
+
+  abbreviation supertypes_of :: "name \<Rightarrow> name list" where
+    "supertypes_of \<equiv> reachable_nodes ty_decl"
+
+  abbreviation (input) type_predatm :: "'a \<Rightarrow> name \<Rightarrow> 'a atom" where
+    "type_predatm x t \<equiv> predAtm (pred_for_type t) [x]"
+
+  fun type_atom :: "'a \<Rightarrow> name \<Rightarrow> 'a atom formula" where
+    "type_atom x t = Atom (type_predatm x t)"
+
+  fun type_precond :: "variable \<times> type \<Rightarrow> term atom formula" where
+    "type_precond (v, (Either ts)) = \<^bold>\<Or> (map (type_atom (term.VAR v)) ts)"
+
+  definition param_precond :: "(variable \<times> type) list \<Rightarrow> term atom formula" where
+    "param_precond params = \<^bold>\<And> (map type_precond params)"
+
+  abbreviation (in -) detype_pred :: "predicate_decl \<Rightarrow> predicate_decl" where
+    "detype_pred p \<equiv> PredDecl (pred p) (replicate (length (predicate_decl.argTs p)) \<omega>)"
+
+  definition (in -) detype_preds :: "predicate_decl list \<Rightarrow> predicate_decl list" where
+    "detype_preds preds \<equiv> map detype_pred preds"
+
+  fun (in -) detype_fun :: "function_decl \<Rightarrow> function_decl" where
+    "detype_fun (FuncDecl n as) = FuncDecl n (replicate (length as) \<omega>)"
+
+  definition (in -) detype_funs :: "function_decl list \<Rightarrow> function_decl list" where
+    "detype_funs funs \<equiv> map detype_fun funs"
+
+  fun (in -) detype_ent :: "('ent \<times> type) \<Rightarrow> ('ent \<times> type)" where
+    "detype_ent (n, T) = (n, \<omega>)"
+
+  definition (in -) detype_ents :: "('ent \<times> type) list \<Rightarrow> ('ent \<times> type) list" where
+    "detype_ents params \<equiv> map detype_ent params"
+
+  fun (in -) detype_action_head::"ast_action_head \<Rightarrow> ast_action_head" where
+    "detype_action_head (ActionHead n params) = ActionHead n (detype_ents params)"
+
+  fun detype_simple_action_body::"ast_action_head \<Rightarrow> ast_simple_action_body \<Rightarrow> ast_simple_action_body" where
+    "detype_simple_action_body h (SimpleActionBody pre eff) = SimpleActionBody (param_precond (parameters h) \<^bold>\<and> pre) eff"
+
+  text \<open>This only works for single types on purpose.\<close>
+  fun supertype_facts_for :: "(object \<times> type) \<Rightarrow> object atom formula list" where
+    "supertype_facts_for (n, Either [t]) =
+      map (type_atom n) (supertypes_of t)" |
+    "supertype_facts_for (n, _) = undefined"
+
+  definition supertype_facts :: "(object \<times> type) list \<Rightarrow> object atom formula list" where
+    "supertype_facts objs \<equiv> concat (map supertype_facts_for objs)"
+end
+
+text \<open>The detyped predicates, functions, constants, and objects.\<close>
+
+definition (in domain_signature) "detyped_predicates \<equiv> type_preds @ detype_preds predicates"
+
+definition (in domain_signature) "detyped_functions \<equiv> detype_funs functions"
+
+definition (in domain_signature) "detyped_consts \<equiv> detype_ents consts"
+
+definition (in problem_signature) "detyped_objs \<equiv> detype_ents objs"
+
+subsection \<open>The signature \<open>*2\<close> locale hierarchy\<close>
+
+text \<open>Relate signatures to their detyped counterparts. Each \<open>*2\<close> locale extends its plain counterpart
+  and adds a \<open>sig2\<close> sublocale interpretation for the detyped signature.\<close>
+
+locale domain_signature2 = domain_signature
+sublocale domain_signature2 \<subseteq>
+  sig2: domain_signature Nil detyped_predicates detyped_functions detyped_consts .
+
+locale wf_domain_signature2 = wf_domain_signature
+sublocale wf_domain_signature2 \<subseteq> domain_signature2 .
+
+locale problem_signature2 = problem_signature
+sublocale problem_signature2 \<subseteq>
+  sig2: problem_signature Nil detyped_predicates detyped_functions detyped_consts detyped_objs .
+sublocale problem_signature2 \<subseteq> domain_signature2 .
+
+locale wf_problem_signature2 = wf_problem_signature
+sublocale wf_problem_signature2 \<subseteq> problem_signature2 .
+sublocale wf_problem_signature2 \<subseteq> wf_domain_signature2 by unfold_locales
+
+text \<open>Now the restricted (no Either types) signatures.\<close>
+
+locale restrict_domain_signature2 = restrict_domain_signature
+sublocale restrict_domain_signature2 \<subseteq> domain_signature2 .
+
+locale restrict_problem_signature2 = restrict_problem_signature
+sublocale restrict_problem_signature2 \<subseteq> problem_signature2 .
+
+locale wf_restrict_domain_signature2 = wf_restrict_domain_signature
+sublocale wf_restrict_domain_signature2 \<subseteq> restrict_domain_signature2 ..
+sublocale wf_restrict_domain_signature2 \<subseteq> wf_domain_signature2 ..
+
+locale wf_restrict_problem_signature2 = wf_restrict_problem_signature
+sublocale wf_restrict_problem_signature2 \<subseteq> restrict_problem_signature2 ..
+sublocale wf_restrict_problem_signature2 \<subseteq> wf_problem_signature2 ..
+sublocale wf_restrict_problem_signature2 \<subseteq> wf_restrict_domain_signature2 ..
+
+end
